theories/Hoare.v
@@ -3,7 +3,9 @@
 (* Adapted from the Software Foundations series:
    https://softwarefoundations.cis.upenn.edu/ *)
 
-Require Import Coq.Program.Tactics.
+Require Import Coq.Program.Tactics
+        Coq.Lists.List.
+
 Require Import Maps Imp HoareCommon.
 
 (* ################################################################# *)
@@ -12,11 +14,11 @@ Require Import Maps Imp HoareCommon.
 Section Hoare.
 
   Reserved Notation "Sigma |- {{ P }}  c  {{ Q }}"
-           (at level 90, c at next level).
+           (at level 40, c at next level).
 
   Inductive hoare_proof (Sigma : total_map funSpec) : Assertion -> com -> Assertion -> Prop :=
   | H_Skip : forall P,
-      Sigma |- {{P}} SKIP {{P}}
+      Sigma |- {{ P }} SKIP {{P}}
   | H_Asgn : forall Q V a,
       Sigma |- {{Q[V |-> a]}} V ::= a {{Q}}
   | H_Seq  : forall P c Q d R,
@@ -46,15 +48,17 @@ Section Hoare.
 where "Sigma |- {{ P }}  c  {{ Q }}" := (hoare_proof Sigma P c Q) : hoare_spec_scope.
 
   Definition hoare_triple
-             {env : Env}
-             (P : Assertion) (c : com) (Q : Assertion) : Prop :=
+             (Sigma : Env)
+             (P : Assertion)
+             (c : com)
+             (Q : Assertion) : Prop :=
     forall st st',
-      st =[ c ]=> st'  ->
+      Sigma |- st =[ c ]=> st'  ->
       P st  ->
       Q st'.
 
-  Notation "{{ P }}  c  {{ Q }}" :=
-    (hoare_triple P c Q) (at level 90, c at next level)
+  Notation "Sigma '|=' {{ P }}  c  {{ Q }}" :=
+    (hoare_triple Sigma P c Q) (at level 40, c at next level)
     : hoare_spec_scope.
 
   Hint Resolve bassn_eval_true bassn_eval_false : hoare.
@@ -62,9 +66,9 @@ where "Sigma |- {{ P }}  c  {{ Q }}" := (hoare_proof Sigma P c Q) : hoare_spec_s
   Hint Unfold hoare_triple.
   Hint Constructors ceval.
 
-  Lemma hoare_while {env : Env} : forall P b c,
-      {{fun st => P st /\ bassn b st}} c {{P}} ->
-      {{P}} WHILE b DO c END {{fun st => P st /\ ~ (bassn b st)}}.
+  Lemma hoare_while (Sigma : Env) : forall P b c,
+      Sigma |= {{fun st => P st /\ bassn b st}} c {{P}} ->
+      Sigma |= {{P}} WHILE b DO c END {{fun st => P st /\ ~ (bassn b st)}}.
   Proof.
     unfold hoare_triple.
     intros ? ? ? ? ? ? HE ?. remember (WHILE b DO c END)%imp eqn:Heq.
@@ -73,9 +77,9 @@ where "Sigma |- {{ P }}  c  {{ Q }}" := (hoare_proof Sigma P c Q) : hoare_spec_s
     - eauto.
   Qed.
 
-  Theorem hoare_proof_sound Sigma : forall P c Q,
+  Theorem hoare_proof_sound Sigs Sigma : forall P c Q,
       Sigma |- {{P}} c {{Q}} ->
-      @hoare_triple {| funSpecs := Sigma; funDefs := empty |} P c Q.
+       {| funSigs := Sigs; funSpecs := Sigma; funDefs := empty |} |= {{P}} c {{Q}}.
   Proof.
   intros ? ? ? pf. induction pf; intros st st' HE HP.
   - (* SKIP *)
@@ -85,28 +89,29 @@ where "Sigma |- {{ P }}  c  {{ Q }}" := (hoare_proof Sigma P c Q) : hoare_spec_s
   - (* ;; *)
     inversion HE; subst. eauto.
   - (* TEST *)
-    inversion HE; subst. eauto.
-    firstorder with hoare.
+    inversion HE; subst; firstorder with hoare.
   - (* WHILE *)
     eapply hoare_while; eauto.
   - (* Conseq *)
     eauto.
   - (* :::= *)
-    inversion HE; subst; try firstorder.
+    inversion HE; subst; firstorder.
     simpl in H4; rewrite apply_empty in H4; discriminate.
   Qed.
 
-  Definition wp {env : Env} (c:com) (Q:Assertion) : Assertion :=
-    fun s => forall s', s =[ c ]=> s' -> Q s'.
+  Definition wp (Sigma : Env)
+             (c : com)
+             (Q : Assertion) : Assertion :=
+    fun s => forall s', Sigma |- s =[ c ]=> s' -> Q s'.
 
-  Lemma wp_is_precondition {env : Env}: forall c Q,
-      {{wp c Q}} c {{Q}}.
+  Lemma wp_is_precondition (Sigma : Env): forall c Q,
+      Sigma |= {{wp Sigma c Q}} c {{Q}}.
   Proof.
     firstorder.
   Qed.
 
-  Lemma wp_is_weakest {env : Env} : forall c Q P',
-      {{P'}} c {{Q}} -> forall st, P' st -> wp c Q st.
+  Lemma wp_is_weakest (Sigma : Env) : forall c Q P',
+      Sigma |= {{P'}} c {{Q}} -> forall st, P' st -> wp Sigma c Q st.
   Proof.
     firstorder.
   Qed.
@@ -114,8 +119,8 @@ where "Sigma |- {{ P }}  c  {{ Q }}" := (hoare_proof Sigma P c Q) : hoare_spec_s
   Hint Resolve wp_is_precondition wp_is_weakest : hoare.
   Hint Unfold wp.
 
-  Theorem hoare_proof_complete Sigma : forall P c Q,
-      @hoare_triple {| funSpecs := Sigma; funDefs := empty |} P c Q->
+  Theorem hoare_proof_complete Sigs Sigma : forall P c Q,
+      {| funSigs := Sigs; funSpecs := Sigma; funDefs := empty |} |= {{P}} c {{Q}} ->
       Sigma |- {{P}} c {{Q}}.
   Proof.
     unfold hoare_triple.
@@ -130,13 +135,13 @@ where "Sigma |- {{ P }}  c  {{ Q }}" := (hoare_proof Sigma P c Q) : hoare_spec_s
       eapply H_Consequence; eauto with hoare.
       simpl. intros. eapply HT; eauto.
     - (* ;; *)
-      apply H_Seq with (@wp {| funSpecs := Sigma; funDefs := empty |} c2 Q); firstorder eauto.
+      apply H_Seq with (@wp {| funSigs := Sigs; funSpecs := Sigma; funDefs := empty |} c2 Q); firstorder eauto.
     - (* IFB *)
       apply H_If.
       + firstorder eauto.
       + apply IHc2. firstorder with hoare.
     - (* WHILE *)
-      eapply H_Consequence with (P':= @wp {| funSpecs := Sigma; funDefs := empty |} (WHILE b DO c END) Q).
+      eapply H_Consequence with (P':= @wp {| funSigs := Sigs; funSpecs := Sigma; funDefs := empty |} (WHILE b DO c END) Q).
       + constructor. firstorder eauto.
       + eauto.
       + firstorder with hoare.
@@ -145,14 +150,176 @@ where "Sigma |- {{ P }}  c  {{ Q }}" := (hoare_proof Sigma P c Q) : hoare_spec_s
   Theorem hoare_proof_link {Sigma : Env}
     : forall (P Q : Assertion) c,
       valid_Env Sigma ->
-      (forall st, P st -> @Safe {| funSpecs := @funSpecs Sigma; funDefs := empty |} c st) ->
+      (forall st, P st -> @Safe {| funSigs := @funSigs Sigma;
+                                   funSpecs := @funSpecs Sigma;
+                                   funDefs := empty |} c st) ->
       funSpecs |- {{P}} c {{Q}} ->
-      @hoare_triple Sigma P c Q.
+      Sigma |= {{P}} c {{Q}}.
   Proof.
     intros.
-    pose proof (hoare_proof_sound _ _ _ _ H0);
+    pose proof (hoare_proof_sound (@funSigs Sigma) _ _ _ _ H0);
       eauto using valid_Env_refine, hoare_proof_sound.
   Qed.
+
+  (*Fixpoint prove_safe_Env
+           (names : list funName)
+           (Sigs : list funSig)
+           (Specs : list funSpec)
+           (Defs : list funDef)
+  : Prop :=
+  match names, Sigs, Specs, Defs with
+  | f :: names', sig :: Sigs', spec :: Specs', fd :: Defs' =>
+    Forall (fun fd' => ~ AppearsIn f (funBody fd)) Defs' /\
+    ~ AppearsIn f (funBody fd) /\
+      (forall orig_args,
+          Specs |- {{ fun st => Forall2 (fun orig arg => st arg = orig)
+                                           orig_args
+                                           args -> pre (funSpecs f) orig_args }}
+                        body
+                        {{ fun st => post (funSpecs f) (aeval st ret) orig_args }})
+
+
+    valid_funDef (build_Env names' Sigs' Specs' Defs')
+                 spec fd
+  | _, _, _, _ => True
+  end.
+
+Fixpoint safe_Env
+           (names : list funName)
+           (Sigs : list funSig)
+           (Specs : list funSpec)
+           (Defs : list funDef)
+  : Prop :=
+  match names, Sigs, Specs, Defs with
+  | f :: names', sig :: Sigs', spec :: Specs', fd :: Defs' =>
+    Forall (fun fd' => ~ AppearsIn f (funBody fd)) Defs' /\
+    ~ AppearsIn f (funBody fd) /\
+    valid_funDef (build_Env names' Sigs' Specs' Defs')
+                 spec fd
+  | _, _, _, _ => True
+  end.
+
+Lemma safe_Env_is_valid
+  : forall (names : list funName)
+           (Sigs : list funSig)
+           (Specs : list funSpec)
+           (Defs : list funDef),
+    NoDup names ->
+    length names = length Sigs ->
+    length names = length Specs ->
+    length names = length Defs ->
+    safe_Env names Sigs Specs Defs ->
+    valid_Env (build_Env names Sigs Specs Defs).
+Proof.
+  induction names; simpl; intros.
+  - unfold valid_Env; unfold build_Env; simpl; intros;
+      compute in H1; discriminate.
+  - destruct Sigs; destruct Specs; destruct Defs; simpl in *;
+      try discriminate; injections.
+    simpl.
+    unfold build_Env; simpl.
+(* This is a straightforward proof. *)
+Admitted.
+
+  Lemma extend_funDefs
+    : forall
+      (Sigma' : Env)
+      (c : com)
+      (st st' : total_map nat)
+      (H : Sigma' |- st =[ c ]=> st')
+      (Sigma : Env)
+      (fd : funDef)
+      (f : String.string),
+      (Safe {| funSigs := funSigs; funSpecs := funSpecs; funDefs := empty |} c st) ->
+      Sigma' = {| funSigs := funSigs;
+                  funSpecs := funSpecs;
+                  funDefs := fun x' : String.string => if String.string_dec f x' then Some fd else funDefs x' |} ->
+      funDefs f = None ->
+      Sigma |- st =[ c ]=> st'.
+  Proof.
+    induction 1; intros; eauto; subst; simpl in *.
+    - inversion X; subst; econstructor; eauto.
+      eapply IHceval2; eauto.
+      eapply X1.
+      admit.
+    - simpl in *.
+
+  (*- find_if_inside; try discriminate; econstructor; eauto.
+    - find_if_inside; injections; eauto.
+      + econstructor; eauto. *)
+  Admitted.
+
+  Lemma hoare_valid_funDef
+    : forall {Sigma : Env} f args body ret,
+      valid_Env Sigma ->
+      funDefs f = None ->
+      (forall orig_args st,
+          (Forall2 (fun orig arg => st arg = orig)
+                   orig_args
+                   args -> pre (funSpecs f) orig_args)
+          -> @Safe {| funSigs := @funSigs Sigma;
+                      funSpecs := @funSpecs Sigma;
+                      funDefs := empty |} body st) ->
+      (forall orig_args,
+          funSpecs |- {{ fun st => Forall2 (fun orig arg => st arg = orig)
+                                           orig_args
+                                           args -> pre (funSpecs f) orig_args }}
+                        body
+                        {{ fun st => post (funSpecs f) (aeval st ret) orig_args }}) ->
+      valid_Env {|
+          funSigs := funSigs;
+          funSpecs := funSpecs;
+                   funDefs := f |-> {| funArgs := args;
+                                       funBody := body;
+                                       funRet := ret |};
+                   funDefs |}.
+  Proof.
+    unfold valid_Env; simpl; unfold update, t_update; intros.
+    find_if_inside; subst; injections.
+    - assert (forall orig_args,
+                 Sigma |= {{ fun st => Forall2 (fun orig arg => st arg = orig)
+                                               orig_args
+                                               args -> pre (funSpecs f0) orig_args}} body
+                       {{fun st : state => post (funSpecs f0) (aeval st ret) orig_args}}) by
+          eauto using hoare_proof_link.
+      unfold valid_funDef, hoare_triple in *; intros.
+      simpl in *; eapply H2 with (st := build_total_map args args0 0); eauto.
+      replace body with (funBody {| funArgs := args; funBody := body; funRet := ret |}) in X by reflexivity.
+      simpl in X.
+      eapply extend_funDefs in X0; eauto.
+    -
+
+
+        inversion X0; subst; eapply E_IfFalse; eauto; congruence.
+
+        econstructor; eauto.
+          eapply IHbody1; eauto; intros; eapply X in H; inversion H; subst; eauto.
+
+
+      + admit.
+      + eauto.
+
+
+    intros.
+    eapply hoare_proof_link
+    - injections.
+      unfold valid_funDef; intros.
+      eapply hoare_proof_sound in H1; unfold hoare_triple in H1;
+        eapply H1 with (st := build_total_map args args0 0); simpl in *; firstorder.
+      admit.
+    - unfold valid_funDef in *; intros.
+      eapply H; eauto.
+
+      Unset Printing Notations.
+      Set Printing Implicit.
+
+
+
+    - injection H2; intros; subst.
+      Focus 2.
+    eapply H in
+    2: eapply H.
+  Abort. *)
 
   (* This one is going to require more care...*)
   Theorem hoare_valid_Env
