theories/RHLE.v
@@ -5,14 +5,6 @@ Require Import
 
 Require Import Maps Imp.
 
-Ltac inv_ceval :=
-  let t H := (inversion H; subst; clear H) in
-  match goal with
-  | H : _ =[ SKIP ]=> _
-                      |- _ => t H
-  | H : _ =[ _;;_ ]=> _ |- _ => t H
-  end.
-
 Require Import HoareCommon Hoare EHoare.
 
 Definition Assertion2 := state -> state -> Prop.
@@ -22,19 +14,19 @@ Definition assert2_implies (P Q : Assertion2) : Prop :=
 
 Section RHLE.
 
-  Definition rhle_triple {env : Env}
+  Definition rhle_triple (Sigma : Env)
              (P : Assertion2) (c1 : com) (c2 : com) (Q : Assertion2) : Prop :=
     forall st1 st2 st1',
-      st1 =[ c1 ]=> st1'  ->
+      Sigma |- st1 =[ c1 ]=> st1'  ->
                     P st1 st2 ->
-                    exists st2' (exe : st2 =[ c2 ]=> st2'), Q st1' st2'.
+                    exists st2' (exe : Sigma |- st2 =[ c2 ]=> st2'), Q st1' st2'.
 
-  Notation "{{ P }}  c1 ~# c2  {[ Q ]}" :=
-    (rhle_triple P c1 c2 Q) (at level 90, c1 at next level, c2 at next level)
+  Notation "Sigma |= {{ P }}  c1 ~# c2  {[ Q ]}" :=
+    (rhle_triple Sigma P c1 c2 Q) (at level 90, c1 at next level, c2 at next level)
     : hoare_spec_scope.
 
   Reserved Notation "Sigma |- {{ P }}  c1 ~# c2  {[ Q ]}"
-           (at level 90, c1 at next level, c2 at next level).
+           (at level 40, c1 at next level, c2 at next level).
 
   Inductive rhle_proof Sigma : Assertion2 -> com -> com -> Assertion2 -> Prop :=
   | RHE_Skip : forall P,
@@ -46,11 +38,11 @@ Section RHLE.
       Sigma |- {{P}} c1 ~# c2;;SKIP {[Q]} ->
       Sigma |- {{P}} c1 ~# c2 {[Q]}
   | RHE_StepL : forall P Q R c1 c2 c3,
-      (forall st2, Sigma |- {{fun st => P st st2}} c1 {{fun st => Q st st2}}) ->
+      (forall st2, hoare_proof Sigma (fun st => P st st2) c1 (fun st => Q st st2)) ->
       Sigma |- {{Q}} c2 ~# c3 {[R]} ->
       Sigma |- {{P}} c1;;c2 ~# c3 {[R]}
   | RHE_StepR : forall P Q R c1 c2 c3,
-      (forall st1, Sigma |- {[fun st => P st1 st]} c2 {[fun st => Q st1 st]}#) ->
+      (forall st1, ehoare_proof Sigma (fun st => P st1 st) c2 (fun st => Q st1 st)) ->
       Sigma |- {{Q}} c1 ~# c3 {[R]} ->
       Sigma |- {{P}} c1 ~# c2;;c3 {[R]}
 
@@ -61,53 +53,54 @@ Section RHLE.
   Hint Unfold rhle_triple hoare_triple ehoare_triple.
   Hint Constructors ceval.
 
-  Ltac apply_sound :=
+  (*Ltac apply_sound :=
     match goal with
     | H : context[_ |- {{_}} _ {{_}}] |- _ =>
       eapply hoare_proof_sound in H
     | H : context[_ |- {[_]} _ {[_]}#] |- _ =>
       eapply ehoare_proof_sound in H
-    end.
+    end. *)
 
-  Theorem rhle_proof_sound Sigma : forall P c1 c2 Q,
+  Theorem rhle_proof_sound Sigs Sigma : forall P c1 c2 Q,
       Sigma |- {{P}} c1 ~# c2 {[Q]} ->
-      @rhle_triple {| funSpecs := Sigma; funDefs := empty |} P c1 c2 Q.
+      {| funSigs := Sigs; funSpecs := Sigma; funDefs := empty |} |= {{P}} c1 ~# c2 {[Q]}.
   Proof.
     intros ? ? ? ? pf.
     unfold rhle_triple.
     induction pf; intros st1 st2 st1' exe HP.
-    - inv_ceval. eauto.
+    - inversion exe; subst; eauto.
     - firstorder eauto.
     - edestruct IHpf as [st2' [exe' HQ]]; eauto.
-      inv_ceval. inv_ceval. eauto.
-    - inv_ceval. edestruct IHpf; eauto.
-      apply_sound. eauto.
-    - apply_sound.
+      inversion exe'; subst; eauto.
+      inversion X0; subst.
+      eexists _, X; eauto.
+    - inversion exe; subst; edestruct IHpf; eauto.
+      eapply hoare_proof_sound in H; eauto.
+    - eapply ehoare_proof_sound in H; eauto.
       edestruct H as [st' [exe' HQ]]; eauto.
       edestruct IHpf as [st2' [? ?]]; eauto.
   Qed.
 
-  Definition rwp {env : Env} c (Q : Assertion2) : Assertion2 :=
-    fun st1 st2 => exists st2' (exe : st2 =[ c ]=> st2'), Q st1 st2'.
+  Definition rwp (Sigma : Env) c (Q : Assertion2) : Assertion2 :=
+    fun st1 st2 => exists st2' (exe : Sigma |- st2 =[ c ]=> st2'), Q st1 st2'.
 
-  Theorem rhle_proof_complete Sigma : forall P c1 c2 Q,
-      @rhle_triple {| funSpecs := Sigma; funDefs := empty |} P c1 c2 Q -> 
+  Theorem rhle_proof_complete Sigs Sigma : forall P c1 c2 Q,
+      {| funSigs := Sigs; funSpecs := Sigma; funDefs := empty |} |= {{P}} c1 ~# c2 {[Q]} ->
       Sigma |- {{P}} c1 ~# c2 {[Q]}.
   Proof.
     unfold rhle_triple.
     intros P c1 c2 Q H.
-    apply RHE_SkipIntroL. apply RHE_StepL with (@rwp {| funSpecs := Sigma; funDefs := empty |} c2 Q).
-    intros st2. apply hoare_proof_complete.
-    firstorder.
-    apply RHE_SkipIntroR. eapply RHE_StepR. 2: constructor.
-    intros st1. apply ehoare_proof_complete.
-    firstorder.
+    apply RHE_SkipIntroL.
+    apply RHE_StepL with (@rwp {| funSigs := Sigs; funSpecs := Sigma; funDefs := empty |} c2 Q).
+    - intros st2. eapply hoare_proof_complete with (Sigs := Sigs); firstorder.
+    - apply RHE_SkipIntroR. eapply RHE_StepR. 2: constructor.
+      intros st1. apply ehoare_proof_complete with (Sigs := Sigs); firstorder.
   Qed.
 
 End RHLE.
 
-Notation "{{ P }}  c1 ~# c2  {[ Q ]}" :=
-  (rhle_triple P c1 c2 Q) (at level 90, c1 at next level, c2 at next level)
+Notation "Sigma |= {{ P }}  c1 ~# c2  {[ Q ]}" :=
+  (rhle_triple Sigma P c1 c2 Q) (at level 90, c1 at next level, c2 at next level)
   : hoare_spec_scope.
 
 Notation "Sigma |- {{ P }}  c1 ~# c2  {[ Q ]}" :=
